add checks for solver binary present, remove config prints, add comparison to hammer/crush for SearchTree

benchmarking/get_stats.py
@@ -4,221 +4,160 @@ from dataclasses import dataclass
 
 import re
 import sys
+import os
 
-from enum import Enum
-
+from typing import Any, Optional
 
 @dataclass
-class HammerStats:
-  proof_size: int
+class GoalTally:
+  completed: int
   total: int
-  finished: int
 
-  def empty(): return HammerStats(0, 0, 0)
-
-  def merge(self, r):
-    return HammerStats(
-        proof_size=self.proof_size + r.proof_size
-      , total=self.total + r.total
-      , finished=self.finished + r.finished
-    )
-
-  def heading():
-    return f"Hammer Proof, Hammer Total, Hammer Success"
   def pretty(self):
-    return f"{self.proof_size}, {self.total}, {self.finished}"
+    return f"{self.completed}/{self.total}"
 
-@dataclass 
-class ProofStats:
-  defn_size : int
-  manual_size: int
-  hammer: HammerStats
-  ms_size: int
-  ms_success: int
-  
-  def empty(): return ProofStats(0, 0, HammerStats.empty(), 0, 0)
+  @staticmethod
+  def empty():
+    return GoalTally(completed=0, total=0)
 
-  def merge(self, r):
-    return ProofStats(
-        defn_size=self.defn_size + r.defn_size
-      , manual_size=self.manual_size + r.manual_size
-      , hammer=self.hammer.merge(r.hammer)
-      , ms_size=self.ms_size + r.ms_size
-    )
-  def heading():
-    return f"Proof Definition, Manual Proof, {HammerStats.heading()}, MirrorSolve Proof, MirrorSolve Success"
-  def pretty(self):
-    return f"{self.defn_size}, {self.manual_size}, {self.hammer.pretty()}, {self.ms_size}, {self.ms_success}"
+  def __add__(self, rhs:Any):
+    return GoalTally(completed=self.completed + rhs.completed, total=self.total + rhs.total)
+
 
 @dataclass
-class BoilerStats:
-  fol_defn: int
-  uf_axioms: int
-  quoting: int
-  plugin: int
+class ProverTally:
+  crush: GoalTally
+  hammer: GoalTally
+  mirror: GoalTally
 
-  def merge(self, r):
-    return BoilerStats(
-        fol_defn=self.fol_defn + r.fol_defn
-      , uf_axioms=self.uf_axioms + r.uf_axioms
-      , plugin=self.plugin + r.plugin
-      , quoting=self.quoting + r.quoting
-    )
-  # def heading():
-  #   return f"Implementation, {ProofStats.heading()}, {ConfigStats.heading()}"
-  # def pretty(self):
-  #   return f"{self.impl_size}, {self.proof.pretty()}, {self.config.pretty()}"
-
-@dataclass
-class ConfigStats:
-  plugin_size: int
-  tactics_size: int
-  # boilerplate: BoilerStats
-  boilerplate : int
-
-  def empty(): return ConfigStats(0, 0, 0)
-
-  def merge(self, r):
-    return ConfigStats(
-        plugin_size=self.plugin_size + r.plugin_size
-      , tactics_size=self.tactics_size + r.tactics_size
-      # , boilerplate=self.boilerplate.merge(r.plugin)
-      , boilerplate=self.boilerplate + r.boilerplate
-    )
-
-  def heading():
-    return f"Plugins, Tactics, Boilerplate"
   def pretty(self):
-    return f"{self.plugin_size}, {self.tactics_size}, {self.boilerplate}"
+    return f"{self.crush.pretty()}, {self.hammer.pretty()}, {self.mirror.pretty()}"
 
-@dataclass
-class BenchStats:
-  impl_size : int
-  proof: ProofStats
-  config: ConfigStats
+  @staticmethod
+  def empty():
+    return ProverTally(crush=GoalTally.empty(), hammer=GoalTally.empty(), mirror=GoalTally.empty())
 
-  def empty(): return BenchStats(0, ProofStats.empty(), ConfigStats.empty())
-
-  def merge(self, r):
-    return BenchStats(
-        impl_size=self.impl_size + r.impl_size
-      , proof=self.proof.merge(r.proof)
-      , config=self.config.merge(r.config)
+  def __add__(self, rhs:Any):
+    return ProverTally(
+      crush=self.crush + rhs.crush, 
+      hammer=self.hammer + rhs.hammer,
+      mirror=self.mirror + rhs.mirror
     )
 
-  def heading():
-    return f"Implementation, {ProofStats.heading()}, {ConfigStats.heading()}"
-  def pretty(self):
-    return f"{self.impl_size}, {self.proof.pretty()}, {self.config.pretty()}"
 
-def read_file(f_name: str, stats: BenchStats):
+
+def make_header():
+  return "File, Crush completed/total, Hammer completed/total, MirrorSolve completed/total"
+
+def pretty_row(x: ProverTally):
+  return x.pretty()
+
+# gather up stats for crush/hammer/mirrorsolve and count solved/total at the goal level, i.e. 15/16 is 15 of 16 goals solved
+def read_file_goals(f_name: str, keep_field: Optional[str] = None) -> ProverTally:
+  stats = ProverTally.empty()
   with open(f_name) as f:
-    counter = 0
-    lineno = 0
-    reading = False
-    old_payload = None
-    for line in f:
-      lineno += 1
+    for lineno, line in enumerate(f, start=1):
       line = line.strip()
       ms_prefix_re = r"\(\*\*\* MS"
       ms_prefix_match = re.match(ms_prefix_re, line)
-      if ms_prefix_match:
-        rest = line[ms_prefix_match.end():].split()
-        match rest[0]:
-          case "BEGIN":
-            if reading:
-              print(f"double open at {lineno}, exiting early")
-              return stats
-            else:
-              reading = True
-              val = ' '.join(rest[1:-1])
-              payload = eval(val)
-              assert "type" in payload, f"missing type in payload at {lineno}"
-              match payload["type"]:
-                case "configuration":
-                  assert "config_type" in payload, f"missing config_type in payload at {lineno}"
-                  match payload["config_type"]:
-                    case "boilerplate" | "plugin" | "tactics":
-                      old_payload = payload
-                    case _ : 
-                      print(f"""unrecogized reading state {payload["config_type"]} at {lineno}""")
-                      reading = False
-                case "proof":
-                  assert "proof_type" in payload, f"missing proof_type in payload at {lineno}"
-                  match payload["proof_type"]:
-                    case "manual" | "hammer" | "mirrorsolve":
-                      old_payload = payload
-                    case _ : 
-                      print(f"""unrecogized reading state {payload["proof_type"]} at {lineno}""")
-                      reading = False
-                case "proof_definition" | "definition":
-                  old_payload = payload
-                case _:
-                  print(f"""unhandled payload type {payload["type"]} at {lineno}""")
-                  reading = False       
-          case "END":
-            if not reading:
-              print(f"unmatched close at {lineno}, exiting early")
-              return stats
-            else:
-              old_counter = counter
-              counter = 0
-              reading = False
-              val = ' '.join(rest[1:-1])
-              payload = eval(val)
-              assert old_payload == payload, f"inconsistent payloads at {lineno}: {old_payload} vs {payload}"
-              assert "type" in payload, f"missing type in payload at {lineno}"
-              match old_payload["type"]:
-                case "configuration":
-                  match old_payload["config_type"]:
-                    case "boilerplate":
-                      stats.config.boilerplate += old_counter
-                    case "plugin":
-                      stats.config.plugin_size += old_counter
-                    case "tactics":
-                      stats.config.tactics_size += old_counter
-                    case _:
-                      assert False, f"""unmatched payload {old_payload["config_type"]}"""
-                case "proof":
-                  match old_payload["proof_type"]:
-                    case "manual":
-                      stats.proof.manual_size += old_counter
-                    case "hammer":
-                      stats.proof.hammer.proof_size += old_counter
-                      stats.proof.hammer.total += int(old_payload["total"])
-                      stats.proof.hammer.finished += int(old_payload["finished"])
-                    case "mirrorsolve":
-                      stats.proof.ms_size += old_counter
-                      assert "total" in old_payload, f"missing total in ms payload at {lineno}"
-                      stats.proof.ms_success += old_payload["total"]
-                    case _:
-                      assert False
-                case "proof_definition":
-                  stats.proof.defn_size += old_counter
-                case "definition":
-                  stats.impl_size += old_counter
-                case _:
-                  print(f"""unhandled payload type {payload["type"]} at {lineno}""")
-          case "STOP":
-            print(f"stopping early at {lineno}")
-            return stats
-          case _:
-            assert False, f"unhandled tag {rest[0]} at {lineno}"
-      else:
-        if reading: counter += 1
+
+      if not ms_prefix_match:
+        continue
+
+      rest = line[ms_prefix_match.end():].split()
+      match rest[0]:
+        case "LEMMA":
+          val = ' '.join(rest[1:-1])
+          try:
+            payload = eval(val)
+
+            if keep_field and not payload[keep_field]:
+              continue
+
+            total = payload["goals"]
+            ms_res = GoalTally(completed=payload["ms"], total=total)
+            crush_res = GoalTally(completed=payload["crush"], total=total)
+            hammer_res = GoalTally(completed=payload["hammer"], total=total)
+
+            stats += ProverTally(mirror=ms_res, crush=crush_res, hammer=hammer_res)
+
+          except Exception as e:
+            print(f"malformed payload at {lineno}: {val}")
+            print(e)
   return stats
 
+# gather up stats for crush/hammer/mirrorsolve and count solved/total at the lemma level, i.e. 15/16 is 15 of 16 lemmas completely solved
+def read_file_lemmas(f_name: str, keep_field: Optional[str] = None) -> ProverTally:
+  stats = ProverTally.empty()
+  with open(f_name) as f:
+    for lineno, line in enumerate(f, start=1):
+      line = line.strip()
+      ms_prefix_re = r"\(\*\*\* MS"
+      ms_prefix_match = re.match(ms_prefix_re, line)
+
+      if not ms_prefix_match:
+        continue
+
+      rest = line[ms_prefix_match.end():].split()
+      match rest[0]:
+        case "LEMMA":
+          val = ' '.join(rest[1:-1])
+          try:
+            payload = eval(val)
+
+            if keep_field and not payload[keep_field]:
+              continue
+
+            total = payload["goals"]
+            ms_completed = 1 if payload["ms"] == total else 0
+            crush_completed = 1 if payload["crush"] == total else 0
+            hammer_completed = 1 if payload["hammer"] == total else 0
+
+            ms_res = GoalTally(completed=ms_completed, total=1)
+            crush_res = GoalTally(completed=crush_completed, total=1)
+            hammer_res = GoalTally(completed=hammer_completed, total=1)
+
+
+
+            stats += ProverTally(mirror=ms_res, crush=crush_res, hammer=hammer_res)
+
+          except Exception as e:
+            print(f"malformed payload at {lineno}: {val}")
+            print(e)
+  return stats
 
 if __name__ == "__main__":
 
   files = sys.argv
 
-  stats = BenchStats.empty()
+  print("Goals, original:")
+
+  print(make_header())
 
   for fl in sys.argv[1:]:
-    print(f"reading stats from {fl}:")
-    stats = read_file(fl, stats)
+    stats = read_file_goals(fl, "original")
+    print(f"{os.path.basename(fl)}, {pretty_row(stats)}")
 
-  print("overall stats:")
-  print(BenchStats.heading())
-  print(stats.pretty())
+print("Goals, total:")
+
+print(make_header())
+
+for fl in sys.argv[1:]:
+  stats = read_file_goals(fl)
+  print(f"{os.path.basename(fl)}, {pretty_row(stats)}")
+
+print("Lemmas, original:")
+
+print(make_header())
+
+for fl in sys.argv[1:]:
+  stats = read_file_lemmas(fl, "original")
+  print(f"{os.path.basename(fl)}, {pretty_row(stats)}")
+
+print("Lemmas, total:")
+
+print(make_header())
+
+for fl in sys.argv[1:]:
+  stats = read_file_lemmas(fl)
+  print(f"{os.path.basename(fl)}, {pretty_row(stats)}")
